<?xml version="1.0"?>
<rdf:RDF xmlns="http://terminologies.gfbio.org/terms/cafe#"
     xml:base="http://terminologies.gfbio.org/terms/cafe"
     xmlns:rdf="http://www.w3.org/1999/02/22-rdf-syntax-ns#"
     xmlns:owl="http://www.w3.org/2002/07/owl#"
     xmlns:xml="http://www.w3.org/XML/1998/namespace"
     xmlns:xsd="http://www.w3.org/2001/XMLSchema#"
     xmlns:rdfs="http://www.w3.org/2000/01/rdf-schema#">
    <owl:Ontology rdf:about="http://terminologies.gfbio.org/terms/cafe"/>
    

    <!-- http://terminologies.gfbio.org/terms/cafe#isCharacterizedBy -->

    <owl:ObjectProperty rdf:about="http://terminologies.gfbio.org/terms/cafe#isCharacterizedBy"/>

    <!-- 
    ///////////////////////////////////////////////////////////////////////////////////////
    //
    // Classes
    //
    ///////////////////////////////////////////////////////////////////////////////////////
     -->

    <owl:Class rdf:about="http://terminologies.gfbio.org/terms/cafe#Cafe">
	<rdfs:comment xml:lang="en"> 
	  The Cafe element is the root element of the Comprehensive Annotation
	  for Ecology schema.
	</rdfs:comment>
        <rdfs:label xml:lang="en">Cafe</rdfs:label>
    </owl:Class>

    <owl:Class rdf:about="http://terminologies.gfbio.org/terms/cafe#Object">
	<rdfs:subClassOf rdf:resource="http://terminologies.gfbio.org/terms/cafe#Cafe"/>
	<rdfs:comment xml:lang="en"> 
	  The Object describes one object described via the cafe annotation
	  schema. It contains all the context information the references and
	  the resources.
	</rdfs:comment>
        <rdfs:label xml:lang="en">Object</rdfs:label>
    </owl:Class>

    <owl:Class rdf:about="http://terminologies.gfbio.org/terms/cafe#Contexts">
	<rdfs:subClassOf rdf:resource="http://terminologies.gfbio.org/terms/cafe#Object"/>
	<rdfs:comment xml:lang="en"> 
	  Contexts is a wrapper around search object contexts
	</rdfs:comment>
        <rdfs:label xml:lang="en">Contexts</rdfs:label>
    </owl:Class>

    <owl:Class rdf:about="http://terminologies.gfbio.org/terms/cafe#Context">
	<rdfs:subClassOf rdf:resource="http://terminologies.gfbio.org/terms/cafe#Contexts"/>
	<rdfs:comment xml:lang="en"> 
	  The Contexts capture biologcial context information in different
	  categories These categories are time, space, sphere, orgnism, biome,
	  chemical, method and process.
	</rdfs:comment>
        <rdfs:label xml:lang="en">Context</rdfs:label>
    </owl:Class>

    <owl:Class rdf:about="http://terminologies.gfbio.org/terms/cafe#TimeContext">
	<rdfs:subClassOf rdf:resource="http://terminologies.gfbio.org/terms/cafe#Context"/>
	<!-- <owl:disjointWith rdf:resource="http://terminologies.gfbio.org/terms/cafe#"/> -->
	<rdfs:comment xml:lang="en"> 
	  The time context allows to capture the quantitative and qualitative
	  temporal aspects that describe the the search object.
	</rdfs:comment>
        <rdfs:label xml:lang="en">TimeContext</rdfs:label>
    </owl:Class>

    <owl:Class rdf:about="http://terminologies.gfbio.org/terms/cafe#TimeRanges">
	<rdfs:subClassOf rdf:resource="http://terminologies.gfbio.org/terms/cafe#TimeContext"/>
        <!-- <owl:disjointWith rdf:resource="http://terminologies.gfbio.org/terms/cafe#TheConcept"/> -->
	<rdfs:comment xml:lang="en"> 
	  A wrapper around time ranges
	</rdfs:comment>
        <rdfs:label xml:lang="en">TimeRanges</rdfs:label>
    </owl:Class>

    <owl:Class rdf:about="http://terminologies.gfbio.org/terms/cafe#TimeRange">
	<rdfs:subClassOf rdf:resource="http://terminologies.gfbio.org/terms/cafe#TimeRanges"/>
        <!-- <owl:disjointWith rdf:resource="http://terminologies.gfbio.org/terms/cafe#TheConcept"/> -->
	<rdfs:comment xml:lang="en"> 
	  The time range captures the temporal extent of the search object. If
	  both the start and the end date are equal this represents a point in
	  time.
	</rdfs:comment>
        <rdfs:label xml:lang="en">TimeRange</rdfs:label>
    </owl:Class>

    <owl:Class rdf:about="http://terminologies.gfbio.org/terms/cafe#RangeStart">
	<rdfs:subClassOf rdf:resource="http://terminologies.gfbio.org/terms/cafe#TimeRange"/>
        <!-- <owl:disjointWith rdf:resource="http://terminologies.gfbio.org/terms/cafe#TheConcept"/> -->
	<rdfs:comment xml:lang="en"> 
	  The start of the time range in form of a local date and local time
	  associated with a timezone. This can be e.g. the start of the data
	  aquisition.
	</rdfs:comment>
        <rdfs:label xml:lang="en">RangeStart</rdfs:label>
    </owl:Class>

    <owl:Class rdf:about="http://terminologies.gfbio.org/terms/cafe#DateTime">
        <rdfs:subClassOf rdf:resource="http://terminologies.gfbio.org/terms/cafe#RangeEnd"/>
        <rdfs:subClassOf rdf:resource="http://terminologies.gfbio.org/terms/cafe#RangeStart"/>
        <rdfs:subClassOf>
            <owl:Restriction>
                <owl:onProperty rdf:resource="http://terminologies.gfbio.org/terms/cafe#isCharacterizedBy"/>
                <owl:someValuesFrom rdf:resource="http://terminologies.gfbio.org/terms/cafe#date"/>
            </owl:Restriction>
        </rdfs:subClassOf>
        <rdfs:subClassOf>
            <owl:Restriction>
                <owl:onProperty rdf:resource="http://terminologies.gfbio.org/terms/cafe#isCharacterizedBy"/>
                <owl:someValuesFrom rdf:resource="http://terminologies.gfbio.org/terms/cafe#time"/>
            </owl:Restriction>
        </rdfs:subClassOf>
        <rdfs:subClassOf>
            <owl:Restriction>
                <owl:onProperty rdf:resource="http://terminologies.gfbio.org/terms/cafe#isCharacterizedBy"/>
                <owl:someValuesFrom rdf:resource="http://terminologies.gfbio.org/terms/cafe#timezone"/>
            </owl:Restriction>
        </rdfs:subClassOf>
        <rdfs:comment xml:lang="en"> 
	  This element captures a local time range with date, time and olson
	  timezone
	</rdfs:comment>
        <rdfs:label xml:lang="en">DateTime</rdfs:label>
    </owl:Class>

    <owl:Class rdf:about="http://terminologies.gfbio.org/terms/cafe#date">
	<rdfs:subClassOf rdf:resource="http://terminologies.gfbio.org/terms/cafe#DateTime"/>
        <owl:disjointWith rdf:resource="http://terminologies.gfbio.org/terms/cafe#time"/>
        <owl:disjointWith rdf:resource="http://terminologies.gfbio.org/terms/cafe#timezone"/>
	<rdfs:comment xml:lang="en"> 
	  A single date in form YYYY-MM-DD conform to iso 8601.
	</rdfs:comment>
        <rdfs:label xml:lang="en">date</rdfs:label>
    </owl:Class>

    <owl:Class rdf:about="http://terminologies.gfbio.org/terms/cafe#time">
	<rdfs:subClassOf rdf:resource="http://terminologies.gfbio.org/terms/cafe#DateTime"/>
        <owl:disjointWith rdf:resource="http://terminologies.gfbio.org/terms/cafe#date"/>
        <owl:disjointWith rdf:resource="http://terminologies.gfbio.org/terms/cafe#timezone"/>
	<rdfs:comment xml:lang="en"> 
	  A single time in form HH:MM:SS conform to iso 8601.
	</rdfs:comment>
        <rdfs:label xml:lang="en">time</rdfs:label>
    </owl:Class>

    <owl:Class rdf:about="http://terminologies.gfbio.org/terms/cafe#timezone">
	<rdfs:subClassOf rdf:resource="http://terminologies.gfbio.org/terms/cafe#DateTime"/>
        <owl:disjointWith rdf:resource="http://terminologies.gfbio.org/terms/cafe#date"/>
        <owl:disjointWith rdf:resource="http://terminologies.gfbio.org/terms/cafe#time"/>
	<rdfs:comment xml:lang="en"> 
	  The olson timezone to capture the timezone of the given date and time
	  in the range (e.g. Europe/Berlin)
	</rdfs:comment>
        <rdfs:label xml:lang="en">timezone</rdfs:label>
    </owl:Class>
 

    <owl:Class rdf:about="http://terminologies.gfbio.org/terms/cafe#RangeEnd">
	<rdfs:subClassOf rdf:resource="http://terminologies.gfbio.org/terms/cafe#TimeRange"/>
        <!-- <owl:disjointWith rdf:resource="http://terminologies.gfbio.org/terms/cafe#TheConcept"/> -->
	<rdfs:comment xml:lang="en"> 
	  The end of the time range in form of a local date and local time
	  associated with a timezone. This can be e.g. the end of the data
	  aquisition.
	</rdfs:comment>
        <rdfs:label xml:lang="en">RangeEnd</rdfs:label>
    </owl:Class>

    <owl:Class rdf:about="http://terminologies.gfbio.org/terms/cafe#TimePeriods">
	<rdfs:subClassOf rdf:resource="http://terminologies.gfbio.org/terms/cafe#TimeContext"/>
	<owl:disjointWith rdf:resource="http://terminologies.gfbio.org/terms/cafe#TimeRanges"/>
	<rdfs:comment xml:lang="en"> 
	    The time periods is a wrapper that can contain all sorts of time
	    periods that reference the temporal context of the search object.
	</rdfs:comment>
        <rdfs:label xml:lang="en">TimePeriods</rdfs:label>
    </owl:Class>

    <owl:Class rdf:about="http://terminologies.gfbio.org/terms/cafe#TimePeriod">
	<rdfs:subClassOf rdf:resource="http://terminologies.gfbio.org/terms/cafe#TimePeriods"/>
	<rdfs:comment xml:lang="en"> 
	    The time period contains one possible time period describing the
	    search object.
	</rdfs:comment>
        <rdfs:label xml:lang="en">TimePeriod</rdfs:label>
    </owl:Class>

    <owl:Class rdf:about="http://terminologies.gfbio.org/terms/cafe#GeologicalTimePeriod">
	<rdfs:subClassOf rdf:resource="http://terminologies.gfbio.org/terms/cafe#TimePeriod"/>
	<rdfs:comment xml:lang="en"> 
	    The geological age is a container that holds one of the possible
	    geological ages which is relevant for describing the search object.
	    e.g. a sample that comes from the ordovician time period.
	</rdfs:comment>
        <rdfs:label xml:lang="en">GeologicalTimePeriod</rdfs:label>
    </owl:Class>

    <owl:Class rdf:about="http://terminologies.gfbio.org/terms/cafe#GeologicalEon">
	<rdfs:subClassOf rdf:resource="http://terminologies.gfbio.org/terms/cafe#GeologicalTimePeriod"/>
	<rdfs:comment xml:lang="en"> 
	    The geological eon contextualizing the search object. For example:
	    Phanerozoic, Precambrian.
	</rdfs:comment>
        <rdfs:label xml:lang="en">GeologicalEon</rdfs:label>
    </owl:Class>

    <owl:Class rdf:about="http://terminologies.gfbio.org/terms/cafe#GeologicalEra">
	<rdfs:subClassOf rdf:resource="http://terminologies.gfbio.org/terms/cafe#GeologicalTimePeriod"/>
	<rdfs:comment xml:lang="en"> 
	    The geological era contextualizing the search object. For example:
	    Cenozoic, Mesozoic, Paleozoic.
	</rdfs:comment>
        <rdfs:label xml:lang="en">GeologicalEra</rdfs:label>
    </owl:Class>

    <owl:Class rdf:about="http://terminologies.gfbio.org/terms/cafe#GeologicalPeriod">
	<rdfs:subClassOf rdf:resource="http://terminologies.gfbio.org/terms/cafe#GeologicalTimePeriod"/>
	<rdfs:comment xml:lang="en"> 
	    The geological period contextualizing the search object. For
	    example: Quaternary, Neogene, Paleogene.
	</rdfs:comment>
        <rdfs:label xml:lang="en">GeologicalPeriod</rdfs:label>
    </owl:Class>

    <owl:Class rdf:about="http://terminologies.gfbio.org/terms/cafe#GeologicalEpoch">
	<rdfs:subClassOf rdf:resource="http://terminologies.gfbio.org/terms/cafe#GeologicalTimePeriod"/>
	<rdfs:comment xml:lang="en">
	    The geological epoch contextualizing the search object. For
	    example: Holocene, Pleistocene, Pilocene.
	</rdfs:comment>
	<rdfs:label xml:lang="en">GeologicalEpoch</rdfs:label>
    </owl:Class>

    <owl:Class rdf:about="http://terminologies.gfbio.org/terms/cafe#GeologicalAge">
	<rdfs:subClassOf rdf:resource="http://terminologies.gfbio.org/terms/cafe#GeologicalTimePeriod"/>
	<rdfs:comment xml:lang="en">
	    The geological age contextualizing the search object. For example:
	    Calabrian, Gelasian, Piacenzian.
	</rdfs:comment>
	<rdfs:label xml:lang="en">GeologicalAge</rdfs:label>
    </owl:Class>

    <owl:Class rdf:about="http://terminologies.gfbio.org/terms/cafe#TemporalResolutions">
	<rdfs:subClassOf rdf:resource="http://terminologies.gfbio.org/terms/cafe#TimeContext"/>
	<owl:disjointWith rdf:resource="http://terminologies.gfbio.org/terms/cafe#TimePeriods"/>
	<owl:disjointWith rdf:resource="http://terminologies.gfbio.org/terms/cafe#TimeRanges"/>
	<rdfs:comment xml:lang="en">
	    A wrapper around temporal aspects describing the temporal
	    resolution of the search object.
	</rdfs:comment>
	<rdfs:label xml:lang="en">TemporalResolutions</rdfs:label>
    </owl:Class>

    <owl:Class rdf:about="http://terminologies.gfbio.org/terms/cafe#TemporalResolution">
	<rdfs:subClassOf rdf:resource="http://terminologies.gfbio.org/terms/cafe#TemporalResolutions"/>
	<rdfs:comment xml:lang="en">
	    The temporal resolution caputres the temporal aspects of the setup
	    or study the search object comes from.
	</rdfs:comment>
	<rdfs:label xml:lang="en">TemporalResolution</rdfs:label>
    </owl:Class>

    <owl:Class rdf:about="http://terminologies.gfbio.org/terms/cafe#TemporalExtentType">
	<rdfs:subClassOf rdf:resource="http://terminologies.gfbio.org/terms/cafe#TemporalResolution"/>
	<owl:disjointWith rdf:resource="http://terminologies.gfbio.org/terms/cafe#TemporalResolutionType"/>
	<rdfs:comment xml:lang="en">
	    The temporal extent type is a categorical value that describes the extent of
	    the setup the search object comes from (e.g. Second, Minute, Hour, Day, Week,
	    ...).
	</rdfs:comment>
	<rdfs:label xml:lang="en">TemporalExtentType</rdfs:label>
    </owl:Class>

    <owl:Class rdf:about="http://terminologies.gfbio.org/terms/cafe#TemporalResolutionType">
	<rdfs:subClassOf rdf:resource="http://terminologies.gfbio.org/terms/cafe#TemporalResolution"/>
	<owl:disjointWith rdf:resource="http://terminologies.gfbio.org/terms/cafe#TemporalExtentType"/>
	<rdfs:comment xml:lang="en">
	    The temporal resolution is a categorical value that describes the resolution of
	    the setup the search object comes from (e.g. Second, Minute, Hour, Day, Week,
	    ...).
	</rdfs:comment>
	<rdfs:label xml:lang="en">TemporalResolutionType</rdfs:label>
    </owl:Class>

</rdf:RDF>
